add finvw ; not yet generated

mppa_k1c/PostpassSchedulingOracle.ml
@@ -31,7 +31,7 @@ type real_instruction =
   (* FPU *)
   | Fabsd | Fabsw | Fnegw | Fnegd
   | Faddd | Faddw | Fsbfd | Fsbfw | Fmuld | Fmulw
-  | Fmind | Fminw | Fmaxd | Fmaxw
+  | Fmind | Fminw | Fmaxd | Fmaxw | Finvw
   | Fnarrowdw | Fwidenlwd | Floatwz | Floatuwz | Floatdz | Floatudz | Fixedwz | Fixeduwz | Fixeddz | Fixedudz
   | Fcompw | Fcompd
 
@@ -62,6 +62,7 @@ let arith_rr_real = function
   | Pfabsd ->           Fabsd
   | Pfnegw ->           Fnegw
   | Pfnegd ->           Fnegd
+  | Pfinvw ->           Finvw
   | Pfnarrowdw ->       Fnarrowdw
   | Pfwidenlwd ->       Fwidenlwd
   | Pfloatwrnsz ->      Floatwz
@@ -586,7 +587,7 @@ let rec_to_usage r =
   | Fnegd | Fnegw | Fabsd | Fabsw | Fwidenlwd
   | Fmind | Fmaxd | Fminw | Fmaxw -> alu_lite
   | Fnarrowdw -> alu_full
-  | Faddd | Faddw | Fsbfd | Fsbfw | Fmuld | Fmulw -> mau
+  | Faddd | Faddw | Fsbfd | Fsbfw | Fmuld | Fmulw | Finvw -> mau
 
 
 let real_inst_to_latency = function
@@ -607,7 +608,7 @@ let real_inst_to_latency = function
   | Set -> 4 (* According to the manual should be 3, but I measured 4 *)
   | Icall | Call | Cb | Igoto | Goto | Ret -> 42 (* Should not matter since it's the final instruction of the basic block *)
   | Fnegd | Fnegw | Fabsd | Fabsw | Fwidenlwd | Fnarrowdw -> 1
-  | Faddd | Faddw | Fsbfd | Fsbfw | Fmuld | Fmulw -> 4
+  | Faddd | Faddw | Fsbfd | Fsbfw | Fmuld | Fmulw | Finvw -> 4
 
 let rec_to_info r : inst_info =
   let usage = rec_to_usage r
